Completed steps_union proof in Evalutation.thy
Finished weak left omega algebra file

Models/Evaluation.thy
@@ -17,17 +17,231 @@ lemma \<rho>_iso: "X \<subseteq> Y \<Longrightarrow> \<rho> X \<subseteq> \<rho>
 lemma \<iota>_iso: "X \<subseteq> Y \<Longrightarrow> \<iota> X \<subseteq> \<iota> Y"
   by (metis galois_connection order_refl order_trans)
 
-lemma "\<iota> X \<parallel> \<iota> X = \<iota> X"
-  apply (auto simp add: pow_inv_def shuffle_def tshuffle_words_def image_def)
-  apply (simp add: lefts_def rights_def)
-  defer
-  sledgehammer
+lemma (in complete_lattice) Inf_singleton: "Inf {x} = x"
+  by (smt Inf_empty Inf_insert inf_top_right)
+
+lemma lfinite_or_linfinite: "lfinite xs \<or> \<not> lfinite xs"
+  by metis
+
+lemma [simp]: "(R O S) `` X = S `` (R `` X)"
+  by (auto simp add: image_def)
+
+(* Evaluating finite words *)
 
 definition eval_finite_word :: "'a rel list \<Rightarrow> 'a set \<Rightarrow> 'a set" where
   "eval_finite_word xs H \<equiv> foldr op O xs Id `` H"
 
+lemma Inf_conj: "(\<And>n. P xs n \<Longrightarrow> Q xs n) \<Longrightarrow> Inf {enat n |n. P xs n \<and> Q xs n} = Inf {enat n |n. P xs n}"
+  by (metis (hide_lams, mono_tags))
+
+(* Lemmas about eval_finite_word *)
+
+lemma efw_cons [simp]: "eval_finite_word (x # xs) X = eval_finite_word xs (x `` X)"
+  by (auto simp add: eval_finite_word_def)
+
+lemma efw_Nil [simp]: "eval_finite_word [] X = X"
+  by (simp add: eval_finite_word_def)
+
+lemma efw_empty [simp]: "eval_finite_word X {} = {}"
+  by (simp add: eval_finite_word_def)
+
+lemma efw_union [simp]: "eval_finite_word w (p \<union> q) = eval_finite_word w p \<union> eval_finite_word w q"
+  by (auto simp add: eval_finite_word_def)
+
+lemma efw_append [simp]: "eval_finite_word (xs @ ys) X = eval_finite_word ys (eval_finite_word xs X)"
+  by (induct xs arbitrary: X) simp_all
+
+lemma efw_append_empty: "eval_finite_word xs X = {} \<Longrightarrow> eval_finite_word (xs @ ys) X = {}"
+  by simp
+
+lemma efw_iso: "P \<subseteq> Q \<Longrightarrow> eval_finite_word xs P \<le> eval_finite_word xs Q"
+  by (simp add: eval_finite_word_def) (metis Image_mono order_refl)
+
+lemma Inf_enat_prop: "Inf {enat n|n. P n} = enat n \<Longrightarrow> P n"
+  apply (subgoal_tac "{enat n|n. P n} \<noteq> {}")
+  apply (smt Inf_empty Inf_enat_def Inf_mono LeastI_ex infinity_ileE mem_Collect_eq the_enat.simps)
+  by (metis Inf_empty enat.distinct(1) top_enat_def)
+
+lemma Inf_enat_pred_conj: "Inf {enat n|n. P n} \<le> Inf {enat n|n. P n \<and> Q n}"
+  by (auto intro: Least_le LeastI2 simp add: Inf_enat_def)
+
 definition steps :: "'a rel llist \<Rightarrow> 'a set \<Rightarrow> enat" where
-  "steps xs H \<equiv> inf (llength xs) (Inf {enat n|n. eval_finite_word (list_of (ltake (enat n) xs)) H = {}})"
+  "steps xs H \<equiv> min (llength xs) (Inf {enat n|n. eval_finite_word (list_of (ltake (enat n) xs)) H = {}})"
+
+lemma empty_eval_non_empty: "p \<noteq> {} \<Longrightarrow> eval_finite_word xs p = {} \<Longrightarrow> \<exists>x xs'. xs = x # xs'"
+  by (cases xs) simp_all
+
+lemma ltake_append_Suc [simp]: "ltake (enat n) (ltake (enat (Suc n)) xs) = ltake (enat n) xs"
+  by (metis eSuc_enat ile_eSuc lappend_ltake_enat_ldropn le_cases ltake_all ltake_eq_ltake_antimono ltake_lappend1)
+
+find_theorems "list_of" "op \<frown>"
+  
+
+lemma [simp]: "min n (Suc n) = n"
+  by (simp add: min_def)
+
+lemma efw_Suc:
+  assumes "eval_finite_word (list_of (ltake (enat n) xs)) p = {}"
+  shows "eval_finite_word (list_of (ltake (enat (Suc n)) xs)) p = {}"
+proof -
+  from assms
+  have "eval_finite_word (list_of (ltake (enat n) (ltake (enat (Suc n)) xs))) p = {}"
+    by simp
+  hence "eval_finite_word (list_of (ltake (enat n) (ltake (enat (Suc n)) xs)) @ list_of (ldrop (enat n) (ltake (enat (Suc n)) xs))) p = {}"
+    by (rule efw_append_empty)
+  hence "eval_finite_word (list_of (ltake (enat n) (ltake (enat (Suc n)) xs) \<frown> ldrop (enat n) (ltake (enat (Suc n)) xs))) p = {}"
+    by (simp add: list_of_lappend)
+  thus "eval_finite_word (list_of (ltake (enat (Suc n)) xs)) p = {}"
+    by (metis lappend_ltake_enat_ldropn ldrop.simps(1))
+qed
+
+lemma efw_plus_n:
+  assumes "eval_finite_word (list_of (ltake (enat n) xs)) p = {}"
+  shows "eval_finite_word (list_of (ltake (enat (n + n')) xs)) p = {}"  
+proof (induct n')
+  case 0 show ?case by (simp add: assms)
+next
+  case (Suc n) thus ?case by (metis add_Suc_right efw_Suc)
+qed
+
+definition true_above :: "(nat \<Rightarrow> bool) \<Rightarrow> bool" where
+  "true_above P = (\<forall>n. P n \<longrightarrow> P (Suc n))"
+
+lemma ta_pairs: "true_above P \<Longrightarrow> true_above Q \<Longrightarrow> (\<forall>n. P n \<longrightarrow> Q n) \<or> (\<forall>n. Q n \<longrightarrow> P n)"
+  apply (auto simp add: true_above_def)
+  apply (rename_tac m)
+  apply (subgoal_tac "n \<le> m")
+  apply (metis dec_induct)
+  by (metis (full_types) dec_induct le_cases)
+
+lemma conj_simpN1: "(\<forall>n. P n \<longrightarrow> Q n) \<Longrightarrow> P n \<and> Q n \<longleftrightarrow> P n" by auto
+lemma conj_simpN2: "(\<forall>n. Q n \<longrightarrow> P n) \<Longrightarrow> P n \<and> Q n \<longleftrightarrow> Q n" by auto
+
+lemma true_above_Inf:
+  assumes "true_above P" and "true_above Q"
+  shows "Inf {enat n|n. P n \<and> Q n} = Inf {enat n|n. P n} \<or> Inf {enat n|n. P n \<and> Q n} = Inf {enat n|n. Q n}"
+  apply (rule disjE[OF ta_pairs[OF assms(1) assms(2)]])
+  apply (subst conj_simpN1[where P = P and Q = Q])
+  apply simp
+  apply simp
+  apply (subst conj_simpN2[where P = P and Q = Q]) back
+  by auto
+
+lemma true_above_Inf1:
+  assumes "true_above P" and "true_above Q"
+  and "Inf {enat n |n. P n} \<le> Inf {enat n |n. Q n}"
+  shows "Inf {enat n|n. P n \<and> Q n} = Inf {enat n|n. Q n}"
+proof -
+  {
+    assume "Inf {enat n|n. P n \<and> Q n} = Inf {enat n|n. Q n}"
+    hence ?thesis
+      by simp
+  }
+  moreover
+  {
+    assume case2: "Inf {enat n|n. P n \<and> Q n} = Inf {enat n|n. P n}"
+    have "Inf {enat n |n. Q n} \<le> Inf {enat n|n. Q n \<and> P n}"
+      by (rule Inf_enat_pred_conj)
+    also have "... = Inf {enat n|n. P n}"
+      by (simp add: case2 conj_commute)
+    finally have ?thesis using case2 assms(3)
+      by simp
+  }
+  ultimately show ?thesis
+    using true_above_Inf[OF assms(1) assms(2)] by blast
+qed
+
+lemma true_above_Inf2:
+  assumes "true_above P" and "true_above Q"
+  and "Inf {enat n |n. Q n} \<le> Inf {enat n |n. P n}"
+  shows "Inf {enat n|n. P n \<and> Q n} = Inf {enat n|n. P n}"
+proof -
+  {
+    assume "Inf {enat n|n. P n \<and> Q n} = Inf {enat n|n. P n}"
+    hence ?thesis
+      by simp
+  }
+  moreover
+  {
+    assume case2: "Inf {enat n|n. P n \<and> Q n} = Inf {enat n|n. Q n}"
+    have "Inf {enat n |n. P n} \<le> Inf {enat n|n. P n \<and> Q n}"
+      by (rule Inf_enat_pred_conj)
+    also have "... = Inf {enat n|n. Q n}"
+      by (simp add: case2 conj_commute)
+    finally have ?thesis using case2 assms(3)
+      by simp
+  }
+  ultimately show ?thesis
+    using true_above_Inf[OF assms(1) assms(2)] by blast
+qed
+
+lemma efw_true_above: "true_above (\<lambda>n. eval_finite_word (list_of (ltake (enat n) xs)) p = {})"
+  by (auto simp add: true_above_def efw_Suc)
+
+lemma steps_union:
+  assumes "steps xs p = n" and "steps xs q = m"
+  shows "steps xs (p \<union> q) = max n m"
+proof -
+  {
+    assume "n \<le> m" and "Inf {enat n |n. eval_finite_word (list_of (ltake (enat n) xs)) p = {}} \<le> llength xs"
+    hence "steps xs q = steps xs (p \<union> q)"
+      apply (simp add: steps_def assms(1)[symmetric] assms(2)[symmetric])
+      apply (rule arg_cong) back
+      apply (subst true_above_Inf1[OF efw_true_above efw_true_above])
+      apply simp_all
+      by (metis (lifting) min_max.inf_absorb1 min_max.inf_commute)
+    hence ?thesis
+      by (metis `n \<le> m` assms(2) min_max.sup_absorb2)
+  }
+  moreover
+  {
+    assume "m \<le> n" and "Inf {enat n |n. eval_finite_word (list_of (ltake (enat n) xs)) q = {}} \<le> llength xs"
+    hence "steps xs p = steps xs (p \<union> q)"
+      apply (simp add: steps_def assms(1)[symmetric] assms(2)[symmetric])
+      apply (rule arg_cong) back
+      apply (subst true_above_Inf2[OF efw_true_above efw_true_above])
+      apply simp_all
+      by (metis (lifting) min_absorb2)
+    hence ?thesis
+      by (metis `m \<le> n` assms(1) min_max.sup_absorb1)
+  }
+  moreover
+  {
+    assume case3: "llength xs \<le> Inf {enat n |n. eval_finite_word (list_of (ltake (enat n) xs)) p = {}}"
+    and "llength xs \<le> Inf {enat n |n. eval_finite_word (list_of (ltake (enat n) xs)) q = {}}"
+    hence "n = llength xs" and "m = llength xs"
+      using assms(1) assms(2)
+      apply -
+      apply (simp_all add: steps_def)
+      by (metis (lifting) min_max.inf_absorb1)+
+    moreover have "steps xs (p \<union> q) = llength xs"
+      apply (simp add: steps_def)
+      apply (rule min_absorb1)
+      apply (rule order_trans[OF case3])
+      by (rule Inf_enat_pred_conj)
+    ultimately have ?thesis
+      by simp
+  }
+  moreover have "n \<le> m \<and> Inf {enat n |n. eval_finite_word (list_of (ltake (enat n) xs)) p = {}} \<le> llength xs \<or>
+    m \<le> n \<and> Inf {enat n |n. eval_finite_word (list_of (ltake (enat n) xs)) q = {}} \<le> llength xs \<or>
+    llength xs \<le> Inf {enat n |n. eval_finite_word (list_of (ltake (enat n) xs)) p = {}} \<and>
+    llength xs \<le> Inf {enat n |n. eval_finite_word (list_of (ltake (enat n) xs)) q = {}}"
+    by (simp only: assms(1)[symmetric] assms(2)[symmetric] steps_def) (metis (lifting) min_def min_max.inf_le1)
+  ultimately show ?thesis
+    by blast
+qed
+
+lemma steps_LNil [simp]: "steps LNil H = 0"
+  by (simp add: steps_def)
+
+lemma steps_empty [simp]: "steps xs {} = 0"
+  apply (simp add: steps_def eval_finite_word_def)
+  apply (subgoal_tac "0 \<in> {n'. \<exists>n. n' = enat n}")
+  apply (metis (mono_tags) Inf_insert inf_enat_def insert_absorb min_enat_simps(2) min_enat_simps(3))
+  by (simp add: zero_enat_def)
+
+lemma steps_mono: "P \<subseteq> Q \<Longrightarrow> steps xs P \<le> steps xs Q"
+  by (auto intro!: order_trans[OF min_max.inf_le2] Inf_superset_mono simp add: steps_def eval_finite_word_def)
 
 datatype 'a top = Top | NotTop 'a
 
@@ -151,45 +365,8 @@ definition llist_nabla :: "'a rel llist \<Rightarrow> 'a set" where
 definition nabla :: "'a rel lan \<Rightarrow> 'a set top" ("\<nabla>_" [1000] 1000)  where
   "\<nabla>X = NotTop (\<Union>{llist_nabla xs|xs. xs \<in> X})"
 
-lemma steps_LNil: "steps LNil H = 0"
-  by (simp add: steps_def) (metis bot_enat_def inf_bot_left)
-
-lemma steps_empty: "steps xs {} = 0"
-  apply (simp add: steps_def eval_finite_word_def)
-  apply (subgoal_tac "0 \<in> {n'. \<exists>n. n' = enat n}")
-  apply (metis (mono_tags) Inf_insert inf_enat_def insert_absorb min_enat_simps(2) min_enat_simps(3))
-  by (simp add: zero_enat_def)
-
 lemma steps_mono: "P \<subseteq> Q \<Longrightarrow> steps xs P \<le> steps xs Q"
-  by (auto intro!: order_trans[OF inf_sup_ord(2)] Inf_superset_mono simp add: steps_def eval_finite_word_def)
-
-lemma eval_finite_word_mono: "P \<subseteq> Q \<Longrightarrow> eval_finite_word xs P \<le> eval_finite_word xs Q"
-  by (simp add: eval_finite_word_def) (metis Image_mono order_refl)
-
-lemma Inf_enat_prop: "Inf {enat n|n. P n} = enat n \<Longrightarrow> P n"
-  apply (subgoal_tac "{enat n|n. P n} \<noteq> {}")
-  apply (smt Inf_empty Inf_enat_def Inf_mono LeastI_ex infinity_ileE mem_Collect_eq the_enat.simps)
-  by (metis Inf_empty enat.distinct(1) top_enat_def)
-
-lemma finite_steps:
-  assumes "steps xs H = enat n"
-  shows "(llength xs = enat n) \<or> (eval_finite_word (list_of (ltake (enat n) xs)) H = {})"
-proof (cases "llength xs \<le> Inf {enat n |n. eval_finite_word (list_of (ltake (enat n) xs)) H = {}}")
-  case True note c = this
-  hence "steps xs H = llength xs"
-    by (simp add: steps_def inf_absorb1[OF c])
-  thus ?thesis
-    by (metis assms)
-next
-  case False
-  hence c: "Inf {enat n |n. eval_finite_word (list_of (ltake (enat n) xs)) H = {}} \<le> llength xs"
-    by (metis (lifting, no_types) le_cases)
-  hence "Inf {enat n |n. eval_finite_word (list_of (ltake (enat n) xs)) H = {}} = enat n"
-    by (simp add: steps_def inf_absorb2[OF c] assms(1)[symmetric])
-  note this = Inf_enat_prop[OF this]
-  thus ?thesis
-    by auto
-qed
+  by (auto intro!: order_trans[OF min_max.inf_le2] Inf_superset_mono simp add: steps_def eval_finite_word_def)
 
 lemma eval_word_mono:
   assumes "P \<subseteq> Q"
@@ -276,12 +453,8 @@ lemma mod_isol: "p \<le> q \<Longrightarrow> x \<Colon> p \<le> x \<Colon> q"
 lemma "sup (x \<Colon> p) (x \<Colon> q) \<le> x \<Colon> sup p q"
   by (rule mono_sup) (auto intro: mod_isol simp add: mono_def)
 
-find_theorems sup "op \<le>"
-
 lemma [simp]: "bind top (eval_word w) = top"
   by (simp add: Top_top[symmetric])
-
-find_theorems sup Sup
 
 lemma "x \<noteq> {} \<Longrightarrow> x \<Colon> top = top"
   by (auto intro!: Sup_top_eq_top simp add: module_def)
@@ -299,12 +472,127 @@ instance enat :: distrib_lattice
   apply (simp add: sup_enat_def inf_enat_def)
   by (metis min_max.sup_inf_distrib1)
 
-lemma eval_finite_take: "steps w p = enat n \<Longrightarrow> eval_finite_word (list_of (ltake (enat n) w)) p = eval_finite_word (list_of w) p"
-  apply (simp add: steps_def)
+instance enat :: complete_distrib_lattice
   sorry
 
 lemma eval_finite_word_union: "eval_finite_word w (p \<union> q) = eval_finite_word w p \<union> eval_finite_word w q"
-  sorry
+  by (auto simp add: eval_finite_word_def)
+
+lemma assumes "steps w p = n" and"steps w q = m" shows "sup n m \<le> steps w (p \<union> q)"
+proof -
+  let ?sp = "{enat n |n. eval_finite_word (list_of (ltake (enat n) w)) p = {}}"
+  let ?sq = "{enat n |n. eval_finite_word (list_of (ltake (enat n) w)) q = {}}"
+  let ?spq = "{enat n |n. eval_finite_word (list_of (ltake (enat n) w)) (p \<union> q) = {}}"
+
+  have lem: "?spq = ?sp \<inter> ?sq"
+    by (auto simp only: eval_finite_word_union)
+
+  have "sup n m = sup (inf (llength w) (Inf ?sp)) (inf (llength w) (Inf ?sq))"
+    by (metis assms(1) assms(2) steps_def)
+  also have "... = inf (llength w) (sup (Inf ?sp) (Inf ?sq))"
+    by (simp only: inf_sup_distrib1[symmetric])
+  also have "... \<le> inf (llength w) (Inf (?sp \<inter> ?sq))"
+    by (metis (lifting) inf_mono order_refl less_eq_Inf_inter)
+  also have "... = inf (llength w) (Inf ?spq)"
+    by (metis lem)
+  finally show "sup n m \<le> steps w (p \<union> q)"
+    by (metis steps_def)
+qed
+
+definition true_above :: "(nat \<Rightarrow> bool) \<Rightarrow> bool" where
+  "true_above P = (\<forall>n. P n \<longrightarrow> P (Suc n))"
+
+lemma ta_pairs: "true_above P \<Longrightarrow> true_above Q \<Longrightarrow> (\<forall>n. P n \<longrightarrow> Q n) \<or> (\<forall>n. Q n \<longrightarrow> P n)"
+  apply (auto simp add: true_above_def)
+  apply (rename_tac m)
+  apply (subgoal_tac "n \<le> m")
+  apply (metis dec_induct)
+  by (metis (full_types) dec_induct le_cases)
+
+lemma conj_simpN1: "(\<forall>n. P n \<longrightarrow> Q n) \<Longrightarrow> P n \<and> Q n \<longleftrightarrow> P n" by auto
+lemma conj_simpN2: "(\<forall>n. Q n \<longrightarrow> P n) \<Longrightarrow> P n \<and> Q n \<longleftrightarrow> Q n" by auto
+
+lemma true_above_Inf:
+  assumes "true_above P" and "true_above Q"
+  shows "Inf {enat n|n. P n \<and> Q n} = Inf {enat n|n. P n} \<or> Inf {enat n|n. P n \<and> Q n} = Inf {enat n|n. Q n}"
+  apply (rule disjE[OF ta_pairs[OF assms(1) assms(2)]])
+  apply (subst conj_simpN1[where P = P and Q = Q])
+  apply simp
+  apply simp
+  apply (subst conj_simpN2[where P = P and Q = Q]) back
+  by auto
+
+lemma
+  assumes "true_above P" and "true_above Q"
+  and "Inf {enat n|n. P n} = enat n" and "Inf {enat n|n. Q n} = enat m"
+  shows "Inf {enat n|n. P n \<and> Q n} \<le> enat (max n m)"
+  using true_above_Inf[of P Q]
+  apply (rule disjE)
+  apply (rule assms(1))
+  apply (rule assms(2))
+  apply (simp add: assms(3))
+  by (simp add: assms(4))
+
+lemma [simp]: "(R O S) `` X = S `` (R `` X)"
+  by (auto simp add: image_def)
+
+lemma efw_cons [simp]: "eval_finite_word (x # xs) X = eval_finite_word xs (x `` X)"
+  by (auto simp add: eval_finite_word_def)
+
+lemma efw_Nil [simp]: "eval_finite_word [] X = X"
+  by (simp add: eval_finite_word_def)
+
+lemma efw_empty [simp]: "eval_finite_word X {} = {}"
+  by (simp add: eval_finite_word_def)
+
+lemma efw_append [simp]: "eval_finite_word (xs @ ys) X = eval_finite_word ys (eval_finite_word xs X)"
+  by (induct xs arbitrary: X) simp_all
+
+lemma efw_append_empty: "eval_finite_word xs X = {} \<Longrightarrow> eval_finite_word (xs @ ys) X = {}"
+  by simp
+
+find_theorems list_of lappend
+
+lemma list_of_ltake_Suc_conv_snoc_lnth: "enat n < llength w \<Longrightarrow> list_of (ltake (enat (Suc n)) w) = list_of (ltake (enat n) w) @ [lnth w n]"
+  apply (subst ltake_Suc_conv_snoc_lnth)
+  apply simp
+  apply (subst list_of_lappend)
+  apply (metis enat_ord_code(4) lfinite_ltake)
+  apply (metis lfinite_LCons lfinite_LNil)
+  by simp
+
+lemma assumes "steps w p = enat n" and"steps w q = enat m" shows "steps w (p \<union> q) = enat (max n m)"
+  apply (rule Inf_enat_prop)
+  apply (simp add: steps_def eval_finite_word_union)
+  using assms
+  apply (simp add: steps_def)
+  sledgehammer
+
+proof -
+  have "llength w = enat n \<or> eval_finite_word (list_of (ltake (enat n) w)) p = {}"
+    by (rule finite_steps[OF assms(1)])
+  moreover have "llength w = enat m \<or> eval_finite_word (list_of (ltake (enat m) w)) q = {}"
+    by (rule finite_steps[OF assms(2)])
+  {
+    assume "eval_finite_word (list_of (ltake (enat n) w)) p = {}" and "eval_finite_word (list_of (ltake (enat m) w)) q = {}"
+    hence ?thesis
+    apply (simp add: steps_def eval_finite_word_union)
+    apply (subst inf_absorb2)
+    sledgehammer
+    apply (subst Inf_enat_def)
+
+  let ?sp = "{enat n |n. eval_finite_word (list_of (ltake (enat n) w)) p = {}}"
+  let ?sq = "{enat n |n. eval_finite_word (list_of (ltake (enat n) w)) q = {}}"
+  let ?spq = "{enat n |n. eval_finite_word (list_of (ltake (enat n) w)) (p \<union> q) = {}}"
+
+  have lem: "?spq = ?sp \<inter> ?sq"
+    by (auto simp only: eval_finite_word_union)
+
+  have "steps w (p \<union> q) = inf (llength w) (Inf (?sp \<inter> ?sq))"
+    by (simp add: steps_def lem)
+
+lemma eval_finite_take: "steps w p = enat n \<Longrightarrow> eval_finite_word (list_of (ltake (enat n) w)) p = eval_finite_word (list_of w) p"
+oops
 
 lemma eval_word_union: "eval_word w (p \<union> q) = sup (eval_word w p) (eval_word w q)"
 proof -
